\documentclass{article}
\usepackage{graphicx}
\usepackage{amsmath}
\usepackage{pgfplots}
\usepackage{physics}
\usepackage{cancel}
\usepackage{enumitem}
\usepackage{txfonts}

\pgfplotsset{compat=1.18}

\usepackage[a4paper, top=1cm, bottom=2cm, left=2cm, right=2cm, includehead, includefoot]{geometry}

\begin{document}

\noindent
Math 110B - Calculus II  \hfill Prof. Jamey Bass

\noindent\rule{\textwidth}{0.4pt}

\begin{center}
    \textbf{\LARGE Homework 9} \\
    \vspace{12pt}
    \large Aaron W. Tarajos \\
    \textit{\today}
\end{center}

\noindent\rule{\textwidth}{0.4pt}

\section*{11.1 Question 17}
Find a formula for the general term $a_n$, of the sequence, assuming that the pattern of the first few terms continues.
\[
	\left\{ \frac{1}{2},\ -\frac{4}{3},\ \frac{9}{4},\ -\frac{16}{5},\ \frac{25}{6}, \cdots \right\}
\]

\subsection*{Solution}
For all integers \( n \geq 1 \), the general term \( a_n \) of the sequence \( \{ a_n \} \) defined by
\[
\left\{ \frac{1}{2},\ -\frac{4}{3},\ \frac{9}{4},\ -\frac{16}{5},\ \frac{25}{6}, \ldots \right\}
\]
is given by
\begin{equation}
\label{eq:an_formula}
a_n = \frac{(-1)^{n+1} n^2}{n+1}.
\end{equation}

\subsection*{Proof}
Let the denomenator be $b_n \coloneqq n+1$, then we have;
\[
	\{b_n\} = \{ (1+1),(2+1),(3+1),\dots \} = \{2,3,4,5,6,\dots\}
\]
then let the numerator be $c_n \coloneqq n^2$, then;
\[
	\{ c_n \} = \{ (1^2),(2^2),(3^2),\dots \} = \{ 1,4,9,16,25,\dots\}
\]
Lastly the sign of the function is given by $s_n \coloneqq (-1)^{n+1}$;
\[
	\{ s_n \} = \{ (-1)^{1+1},(-1)^{2+1},(-1)^{3+1} \} = \{ 1,-1,1,-1,1,\dots \}
\]
combining these sequences, the $n^{\text{th}}$ term is given by;
\[
	a_n = s_n \frac{c_n}{b_n} = \frac{(-1)^{n+1} n^2}{n+1}
\]

\end{document}
